src/Std/Data/DTreeMap/Internal/WF/Lemmas.lean
@@ -564,6 +564,25 @@ theorem get?_eq_getValueCast? [Ord α] [TransOrd α] [LawfulEqOrd α] {k : α} {
     (hto : t.Ordered) : t.get? k = getValueCast? k t.toListModel := by
   rw [get?_eq_get?ₘ, get?ₘ_eq_getValueCast? hto]
 
+/-!
+''' `get`
+-/
+
+theorem contains_eq_get?ₘ_isSome [Ord α] [TransOrd α] [LawfulEqOrd α] {k : α} {t : Impl α β}
+    (hto : t.Ordered) : containsKey k t.toListModel = (t.get?ₘ k).isSome := by
+  rw [get?ₘ_eq_getValueCast? hto, containsKey_eq_isSome_getValueCast?]
+
+theorem getₘ_eq_getValueCast [Ord α] [TransOrd α] [LawfulEqOrd α] {k : α} {t : Impl α β} (h) {h'}
+    (hto : t.Ordered) : t.getₘ k h' = getValueCast k t.toListModel h := by
+  simp only [getₘ, get?ₘ_eq_getValueCast?]
+  revert h'
+  rw [get?ₘ_eq_getValueCast? hto]
+  · simp [getValueCast?_eq_some_getValueCast ‹_›]
+
+theorem get_eq_getValueCast [Ord α] [TransOrd α] [LawfulEqOrd α] {k : α} {t : Impl α β} {h}
+    (hto : t.Ordered): t.get k h = getValueCast k t.toListModel (contains_eq_containsKey hto ▸ h) := by
+  rw [get_eq_getₘ, get?ₘ_eq_getValueCast? hto]
+
 namespace Const
 
 variable {β : Type v}
